add CODECOPY, comment proofs

EvmMachine.v
@@ -11,67 +11,160 @@ Require Import Instructions.
 Require Import Memory.
 Require Import Stack.
 
-Variable size : nat.
 
-Require Import Vector.
-Variable code : Vector.t instruction size.
-Variable jump_targets : list nat.
-
-
-Definition pc_t := Z.
-Definition inc_pc (pc : pc_t) : pc_t := Z.add pc (1%Z).
-Definition word_to_pc (w : word) : pc_t := Word.intval w.
-Definition pc_to_word (pc : pc_t) : word := Word.repr pc.
-
-Definition exec_jump_instr (i : instruction) (pc : pc_t) (ws : list word) : option (pc_t * list word) :=
-  match i with
-    | I_STOP => Some (pc, ws)
-    | I_JUMP => match ws with
-                  | (to::xs) => Some (word_to_pc to, xs)
-                  | _ => None
-                end
-    | I_JUMPI => match ws with
-                   | (to::cond::xs) => Some (if Word.eq cond Word.zero then (word_to_pc to) else (inc_pc pc), xs)
-                   | _ => None
-                end
-    | I_STACK_ONLY (I_PUSH _) => Some (inc_pc pc, ws) (* depends on code address encoding *)
-    | _ => Some (inc_pc pc, ws)
+Definition exec_mem_instr (i : mem_instruction) (m : memory) (ws : list word) : option (memory * list word) :=
+  match i, ws with
+    | I_MLOAD, addr::ws => Some (m, mem_read_word addr m :: ws )
+    | I_MSTORE, addr::val::ws => Some (mem_store_word addr val m, ws)
+    | I_MSTORE8, addr::val::ws => Some (mem_store_first_byte addr val m, ws)
+    | _, _ => None
   end.
 
-
+(* storage should be indexed by contract id *)
+(* TODO: this is remarkably similar to the interface of CompCerts' Memory.v *)
+Definition exec_storage_instr (i : storage_instruction) (p : storage) (ws : list word) : option (storage * list word) :=
+  match i, ws with
+    | I_SLOAD, addr::ws => Some (p, storage_read addr p :: ws)
+    | I_SSTORE, addr::val::ws => Some (storage_store addr val p, ws)
+    | _, _ => None
+  end.
+Variable c : code.
 Record state := State {
   stack : list word;
   mem : memory;
   stor : storage;
-  pc : Z;
+  pc : pc_t;
 }.
 
 Definition step (i : instruction) st m p pc : option state :=
-  let exec_so := fun i' => match exec_so_instr i' st with
-                             | Some st' => Some (State st' m p pc)
-                             | None => None
-                           end in
+  let mks := fun ost' => match ost' with
+                           | Some st' => Some (State st' m p pc)
+                           | None => None
+                         end in
   match i with
-  | I_STACK_ONLY i' => exec_so i'
+    | I_STACK (I_OP1 op) => mks (apply_1 (eval_op1 op) st)
+    | I_STACK (I_OP2 op) => mks (apply_2 (eval_op2 op) st)
+    | I_STACK (I_OP3 op) => mks (apply_3 (eval_op3 op) st)
+    | I_STACK I_POP => mks (Some (tl st))
+    | I_STACK (I_PUSH  n) => mks (Some (code_read_word_from_n_bytes pc n c::st))
+    | I_STACK (I_DUP n) => mks (dup n st)
+    | I_STACK (I_SWAP n) => mks (swap n st)
 
-  | I_MEMINS i' => match exec_mem_instr i' m st with
-                     | Some (m', st') => Some (State st' m' p pc)
+    | I_MEMINS i' => match exec_mem_instr i' m st with
+                     | Some (m', st') => Some (State st' m' p (inc_pc pc))
                      | None => None
                    end
-  | I_STORINS i' => match exec_storage_instr i' p st with
-                     | Some (p', st') => Some (State st' m p' pc)
+    | I_STORINS i' => match exec_storage_instr i' p st with
+                     | Some (p', st') => Some (State st' m p' (inc_pc pc))
                      | None => None
                    end
 
-  | I_STOP
-  | I_JUMP
-  | I_JUMPI => match exec_jump_instr i pc st with
-                 | Some (pc', st') => Some (State st' m p pc')
-                 | None => None
-               end
-  | I_PC => exec_so (I_PUSH (pc_to_word pc))
-  | I_OTHER _ => None
+    | I_STOP => Some (State st m p pc)
+    | I_JUMP => match st with
+                  | (to::st') => Some (State st' m p to)
+                  | _ => None
+                end
+    | I_JUMPI => match st with
+                   | (to::cond::st') => let pc' := if Word.eq cond Word.zero 
+                                                   then (inc_pc pc)
+                                                   else to
+                                        in Some (State st' m p pc')
+                   | _ => None
+                end
+    | I_PC => mks (Some (pc::st))
+    | I_BLOCK _ => None
+
+    | I_ENV I_ADDRESS => None
+    | I_ENV I_BALANCE => None
+    | I_ENV I_ORIGIN => None
+    | I_ENV I_CALLER => None
+    | I_ENV I_CALLVALUE => None
+    | I_ENV I_CALLDATALOAD => None
+    | I_ENV I_CALLDATASIZE => None
+    | I_ENV I_CALLDATACOPY => None
+    | I_ENV I_CODESIZE => None
+    | I_ENV I_CODECOPY => match st with
+                            | to::from::count::st' => Some (State st' (copy_code_to_memory c m to from count) p pc)
+                            | _ => None
+                          end
+    | I_ENV I_GASPRICE => None
+    | I_ENV I_EXTCODESIZE => None
+    | I_ENV I_EXTCODECOPY => None
+
+    | I_SYS _ => None
+    | I_OTHER _ => None
+    | I_INVALID => None
   end.
+
+(* 
+Lemma exec_mem_nice : forall i m st m' st',
+  exec_mem_instr i m st = Some (m', st') ->
+    st' = firstn (alpha (I_MEMINS i)) st' ++ skipn (delta (I_MEMINS i)) st.
+Proof.
+  intros.
+  destruct (exec_mem_instr i m st) eqn:Q; inversion H.
+  subst.
+  destruct i; repeat (destruct st; inversion Q; try reflexivity).
+Qed.
+
+
+Lemma exec_storage_nice : forall i p st p' st',
+  exec_storage_instr i p st = Some (p', st') ->
+    st' = firstn (alpha (I_STORINS i)) st' ++ skipn (delta (I_STORINS i)) st.
+Proof.
+  intros.
+  destruct (exec_storage_instr i p st) eqn:Q; inversion H.
+  subst.
+  destruct i; repeat (destruct st; inversion Q; try reflexivity).
+Qed.
+
+Lemma exec_so_nice : forall i st st' m p pc,
+  (step (I_STACK i) st m p pc) = Some (State st' m p pc) ->
+    let a := (alpha (I_STACK i)) in
+    let d := (delta (I_STACK i)) in
+    st' = firstn a st' ++ skipn d st.
+Proof.
+  intros.
+  destruct (step (I_STACK i) st m p pc0) eqn:Q; inversion H.
+  subst s.
+  destruct i.
+  + (* I_OP1 *)
+    destruct st; inversion Q.
+    reflexivity.
+  + (* I_OP2 *)
+    destruct st eqn:?. simplify_eq Q.
+    destruct l eqn:?. simplify_eq Q.
+    inversion Q.
+    reflexivity.
+  + (* I_OP3 *)
+    destruct st eqn:?. simplify_eq Q.
+    destruct l eqn:?. simplify_eq Q.
+    destruct l0; inversion Q.
+    reflexivity.
+  + (* I_POP *)
+    simpl in Q. unfold tl in Q.
+    destruct st eqn:?; inversion Q; reflexivity.
+  + (* I_PUSH *)
+    inversion Q.
+    reflexivity.
+  + (* I_DUP *)
+    unfold step in Q. unfold dup in Q.
+    destruct (nth_error st n) eqn:NE; inversion Q.
+    destruct st. destruct n; inversion NE.
+    simpl. f_equal. f_equal.
+    symmetry.
+    apply firstn_skipn.
+  + (* I_SWAP *)
+    simpl in Q.
+    compute in a. subst a.
+    compute in d. subst d.
+    destruct (swap n st) eqn:Q1; inversion Q.
+    apply swap_alpha_2n_delta_2n in Q1. inversion Q. subst l.
+    rewrite <- (firstn_skipn (S (S n)) st') at 1.
+    symmetry.
+    apply f_equal.
+    assumption.
+Qed.
 
 Ltac dis_invert e Q := destruct e; inversion Q; try reflexivity.
 
@@ -81,8 +174,11 @@ Theorem step_nice : forall i st m p pc st' m' p' pc',
 Proof.
   intros.
   destruct i; simpl in H; inversion H; simpl; try reflexivity.
-  - apply exec_so_nice.
-    dis_invert (exec_so_instr s st) H.
+  - simpl in H1.
+    unfold delta, alpha.
+    destruct s. simpl. H. in
+    apply (exe_so_nice s st st' m' p' pc').
+    destruct (step (I_STACK s) st m' p' pc').
   - apply (exec_mem_nice _ m _ m' _).
     dis_invert (exec_mem_instr m0 m st) H.
     dis_invert p0 H.
@@ -93,3 +189,4 @@ Proof.
   - dis_invert st H.
     dis_invert st H.
 Qed.
+*)
