Instructions.v
@@ -1,4 +1,3 @@
-Require Export Word.
 
 Inductive op1 : Type :=
   | OP_ISZERO
@@ -36,9 +35,9 @@ Inductive so_instruction : Type :=
   | I_OP2 : op2 -> so_instruction
   | I_OP3 : op3 -> so_instruction
   | I_POP
-  | I_PUSH : word -> so_instruction (* coerced from a list of 1-32 bytes, big endian; the rest is zero *)
-  | I_DUP (n : nat) : n < 16 -> so_instruction (* n is one less than DUPN *)
-  | I_SWAP (n : nat) : n < 16 -> so_instruction (* n is one less than SWAPN *)
+  | I_PUSH : nat -> so_instruction (* coerced from a list of 1-32 bytes, big endian; the rest is zero *)
+  | I_DUP : nat -> so_instruction
+  | I_SWAP : nat -> so_instruction
 .
 
 Inductive mem_instruction : Type :=
@@ -52,20 +51,29 @@ Inductive storage_instruction : Type :=
   | I_SSTORE
 .
 
-Inductive other_instruction : Type :=
-  | I_SHA3
+Inductive env_instruction : Type :=
   | I_ADDRESS | I_BALANCE | I_ORIGIN
   | I_CALLER | I_CALLVALUE | I_CALLDATALOAD | I_CALLDATASIZE | I_CALLDATACOPY
   | I_CODESIZE | I_CODECOPY | I_GASPRICE | I_EXTCODESIZE | I_EXTCODECOPY
+.
+
+Inductive block_instruction : Type :=
   | I_BLOCKHASH | I_COINBASE | I_TIMESTAMP | I_NUMBER | I_DIFFICULTY | I_GASLIMIT
+.
+
+Inductive system_instruction : Type :=
+  | I_CREATE | I_CALL | I_CALLCODE | I_RETURN | I_DELEGATECALL | I_SUICIDE
+.
+
+Inductive other_instruction : Type :=
+  | I_SHA3
   | I_MSIZE | I_GAS | I_JUMPDEST (* NO-OP - mark as label *)
   | I_LOG : nat (* 0-4 *) -> other_instruction
-  | I_CREATE | I_CALL | I_CALLCODE | I_RETURN | I_DELEGATECALL | I_SUICIDE
 .
 
 Inductive instruction : Type :=
   | I_STOP
-  | I_STACK_ONLY : so_instruction -> instruction
+  | I_STACK : so_instruction -> instruction
   | I_MEMINS : mem_instruction -> instruction
   | I_STORINS : storage_instruction -> instruction
 
@@ -73,42 +81,46 @@ Inductive instruction : Type :=
   | I_JUMPI
   | I_PC
 
+  | I_ENV : env_instruction -> instruction
+  | I_BLOCK : block_instruction -> instruction
+  | I_SYS : system_instruction -> instruction
   | I_OTHER : other_instruction -> instruction
+  | I_INVALID : instruction
 .
 
 
 Definition delta_alpha (i: instruction) : nat*nat :=
   match i with
     | I_STOP => (0, 0)
-    | I_STACK_ONLY (I_OP1 _) => (1, 1)
-    | I_STACK_ONLY (I_OP2 _) => (2, 1)
-    | I_STACK_ONLY (I_OP3 _) => (3, 1)
-    | I_STACK_ONLY I_POP => (1, 0)
-    | I_STACK_ONLY (I_PUSH _) => (0, 1)
-    | I_STACK_ONLY (I_DUP n _) => (1 + n, 2 + n)
-    | I_STACK_ONLY (I_SWAP n _) => (2 + n, 2 + n)
+    | I_STACK (I_OP1 _) => (1, 1)
+    | I_STACK (I_OP2 _) => (2, 1)
+    | I_STACK (I_OP3 _) => (3, 1)
+    | I_STACK I_POP => (1, 0)
+    | I_STACK (I_PUSH n) => (0, 1)
+    | I_STACK (I_DUP n) => (n, 1 + n)
+    | I_STACK (I_SWAP n) => (2 + n, 2 + n)
     | I_OTHER I_SHA3 => (2, 1)
 
-    | I_OTHER I_ADDRESS => (0, 1)
-    | I_OTHER I_BALANCE => (1, 1)
-    | I_OTHER I_ORIGIN => (0, 1)
-    | I_OTHER I_CALLER => (0, 1)
-    | I_OTHER I_CALLVALUE => (0, 1)
-    | I_OTHER I_CALLDATALOAD => (1, 1)
-    | I_OTHER I_CALLDATASIZE => (0, 1)
-    | I_OTHER I_CALLDATACOPY => (3, 0)
-    | I_OTHER I_CODESIZE => (0, 1)
-    | I_OTHER I_CODECOPY => (3, 0)
-    | I_OTHER I_GASPRICE => (0, 1)
-    | I_OTHER I_EXTCODESIZE => (1, 1)
-    | I_OTHER I_EXTCODECOPY => (4, 0)
+    | I_ENV I_ADDRESS => (0, 1)
+    | I_ENV I_BALANCE => (1, 1)
+    | I_ENV I_ORIGIN => (0, 1)
+    | I_ENV I_CALLER => (0, 1)
+    | I_ENV I_CALLVALUE => (0, 1)
+    | I_ENV I_CALLDATALOAD => (1, 1)
+    | I_ENV I_CALLDATASIZE => (0, 1)
+    | I_ENV I_CALLDATACOPY => (3, 0)
+    | I_ENV I_CODESIZE => (0, 1)
+    | I_ENV I_CODECOPY => (3, 0)
+    | I_ENV I_GASPRICE => (0, 1)
+    | I_ENV I_EXTCODESIZE => (1, 1)
+    | I_ENV I_EXTCODECOPY => (4, 0)
 
-    | I_OTHER I_BLOCKHASH => (1, 1)
-    | I_OTHER I_COINBASE => (0, 1)
-    | I_OTHER I_TIMESTAMP => (0, 1)
-    | I_OTHER I_NUMBER => (0, 1)
-    | I_OTHER I_DIFFICULTY => (0, 1)
-    | I_OTHER I_GASLIMIT => (0, 1)
+    | I_BLOCK I_BLOCKHASH => (1, 1)
+    | I_BLOCK I_COINBASE => (0, 1)
+    | I_BLOCK I_TIMESTAMP => (0, 1)
+    | I_BLOCK I_NUMBER => (0, 1)
+    | I_BLOCK I_DIFFICULTY => (0, 1)
+    | I_BLOCK I_GASLIMIT => (0, 1)
 
     | I_MEMINS I_MLOAD => (1, 1)
     | I_MEMINS I_MSTORE => (2, 0)
@@ -126,17 +138,136 @@ Definition delta_alpha (i: instruction) : nat*nat :=
 
     | I_OTHER (I_LOG n) => (n + 2, 0)
 
-    | I_OTHER I_CREATE => (3, 1)
-    | I_OTHER I_CALL => (7, 1)
-    | I_OTHER I_CALLCODE => (7, 1)
-    | I_OTHER I_RETURN => (2, 0)
-    | I_OTHER I_DELEGATECALL => (6, 1)
-    | I_OTHER I_SUICIDE => (1, 10)
+    | I_SYS I_CREATE => (3, 1)
+    | I_SYS I_CALL => (7, 1)
+    | I_SYS I_CALLCODE => (7, 1)
+    | I_SYS I_RETURN => (2, 0)
+    | I_SYS I_DELEGATECALL => (6, 1)
+    | I_INVALID => (0, 0)
+    | I_SYS I_SUICIDE => (1, 10)
   end.
 
-Definition delta (i: instruction) : nat := fst (delta_alpha i).
-Definition alpha (i: instruction) : nat := snd (delta_alpha i).
+Require Import List PeanoNat.
+Import ListNotations.
 
+Local Definition fill16 (l : list instruction) : list instruction:=
+  l ++ repeat I_INVALID (16 - length l).
+
+(* 0s: Stop and Arithmetic Operations *)
+Definition opcode_0s := fill16 [
+ I_STOP;
+
+ I_STACK (I_OP2 OP_ADD);
+ I_STACK (I_OP2 OP_MUL);
+ I_STACK (I_OP2 OP_SUB);
+ I_STACK (I_OP2 OP_DIV);
+ I_STACK (I_OP2 OP_SDIV);
+ I_STACK (I_OP2 OP_MOD);
+ I_STACK (I_OP2 OP_SMOD);
+ I_STACK (I_OP3 OP_ADDMOD);
+ I_STACK (I_OP3 OP_MULMOD);
+ I_STACK (I_OP2 OP_EXP);
+ I_STACK (I_OP2 OP_SIGNEXTEND)
+].
+
+(* 10s: Comparison & Bitwise Logic Operations *)
+Definition opcode_10s := fill16 [
+ I_STACK (I_OP2 OP_LT);
+ I_STACK (I_OP2 OP_GT);
+ I_STACK (I_OP2 OP_SLT);
+ I_STACK (I_OP2 OP_SGT);
+ I_STACK (I_OP2 OP_EQ);
+ I_STACK (I_OP1 OP_ISZERO);
+ I_STACK (I_OP2 OP_AND);
+ I_STACK (I_OP2 OP_OR);
+ I_STACK (I_OP2 OP_XOR);
+ I_STACK (I_OP1 OP_NOT);
+ I_STACK (I_OP2 OP_BYTE)
+].
+
+(* 20s: SHA3 *)
+Definition opcode_20s := fill16 [
+  I_OTHER I_SHA3
+].
+
+(* 30s: Environmental Information *)
+Definition opcode_30s := fill16 [
+ I_ENV I_ADDRESS;
+ I_ENV I_BALANCE;
+ I_ENV I_ORIGIN;
+ I_ENV I_CALLER;
+ I_ENV I_CALLVALUE;
+ I_ENV I_CALLDATALOAD;
+ I_ENV I_CALLDATASIZE;
+ I_ENV I_CALLDATACOPY;
+ I_ENV I_CODESIZE;
+ I_ENV I_CODECOPY;
+ I_ENV I_GASPRICE;
+ I_ENV I_EXTCODESIZE;
+ I_ENV I_EXTCODECOPY
+].
+
+(* 50s: Stack, Memory, Storage and Flow Operations *)
+Definition opcode_40s := fill16 [
+ I_BLOCK I_BLOCKHASH;
+ I_BLOCK I_COINBASE;
+ I_BLOCK I_TIMESTAMP;
+ I_BLOCK I_NUMBER;
+ I_BLOCK I_DIFFICULTY;
+ I_BLOCK I_GASLIMIT
+].
+
+(* 50s: Stack, Memory, Storage and Flow Operations *)
+Definition opcode_50s := fill16 [
+ I_STACK I_POP;
+ I_MEMINS I_MLOAD;
+ I_MEMINS I_MSTORE;
+ I_MEMINS I_MSTORE8;
+ I_STORINS I_SLOAD;
+ I_STORINS I_SSTORE;
+ I_JUMP;
+ I_JUMPI;
+ I_PC;
+ I_OTHER I_MSIZE;
+ I_OTHER I_GAS;
+ I_OTHER I_JUMPDEST
+].
+
+(* f0s: System operations *)
+Definition opcode_f0s := [
+ I_SYS I_CREATE;
+ I_SYS I_CALL;
+ I_SYS I_CALLCODE;
+ I_SYS I_RETURN;
+ I_SYS I_DELEGATECALL
+] ++ repeat I_INVALID 10 ++ [
+ I_SYS I_SUICIDE
+].
+
+
+Definition opcode : list instruction := []
+(* 0 *) ++ opcode_0s
+(* 1 *) ++ opcode_10s
+(* 2 *) ++ opcode_20s
+(* 3 *) ++ opcode_30s
+(* 4 *) ++ opcode_40s
+(* 5 *) ++ opcode_50s
+(* 6 *) ++ map (fun n => I_STACK (I_PUSH n)) (seq 1 16)
+(* 7 *) ++ map (fun n => I_STACK (I_PUSH n)) (seq 17 16)
+(* 8 *) ++ map (fun n => I_STACK (I_DUP n)) (seq 1 16)
+(* 9 *) ++ map (fun n => I_STACK (I_SWAP n)) (seq 1 16)
+(* a *) ++ fill16 (map (fun n => I_OTHER (I_LOG n)) (seq 0 5))
+(* b *) ++ fill16 []
+(* c *) ++ fill16 []
+(* d *) ++ fill16 []
+(* e *) ++ fill16 []
+(* f *) ++ opcode_f0s
+.
+
+Definition delta (i: instruction) := fst (delta_alpha i).
+Definition alpha (i: instruction) := snd (delta_alpha i).
+
+Require Export Word.
 Include Word.Word.
 
 Definition eval_op1 (op : op1) (x : word) : word :=
