Memory.v
@@ -1,17 +1,20 @@
+Require Import List.
 Require Import ZArith.
-Require Coqlib.
 
-Require Import Word.
-Require Import Instructions.
+Require Coqlib.
 Require Import Integers.
 Require Import Maps.
-Require Import List.
+
+Require Import Word.
+
 Import ListNotations.
 
 Module WordMap := ZMap.
 
+Section Memory.
+
 Definition memory := WordMap.t byte.
-Definition mget (addr : word) (m : memory) : byte := (WordMap.get (Word.intval addr) m).
+Definition mem_read_byte (addr : word) (m : memory) : byte := (WordMap.get (Word.intval addr) m).
 
 Definition mem_store_byte (addr : word) (b : byte) (m : memory) : memory :=
   (ZMap.set (Word.intval addr) b m).
@@ -19,34 +22,25 @@ Definition mem_store_byte (addr : word) (b : byte) (m : memory) : memory :=
 Definition mem_store_first_byte (addr : word) (w : word) (m : memory) : memory :=
   (ZMap.set (Word.intval addr) (Byte.repr (Z.modulo (Word.intval w) 256)) m).
 
+Definition mem_read_word_from_n_bytes (addr: word) (n: nat) (m : memory) : word :=
+  Word.word_from_byte_seq (map (fun i => mem_read_byte (add (Word.of_nat i) addr) m) (seq 0 n)).
+
 Definition mem_read_word (addr : word) (m : memory) : word :=
   let b := fun n => WordMap.get (Z.add (Word.intval addr) n) m in
   word_from_bytes (b 0%Z) (b 1%Z) (b 2%Z) (b 3%Z) (b 4%Z) (b 5%Z) (b 6%Z) (b 7%Z).
 
+Local Definition wordadd addr n :=
+  Word.repr (Z.add (Word.intval addr) (Z.of_nat n)).
+
 Definition mem_store_word (w : word) (addr : word) (m : memory) : memory :=
   let '(a0, a1, a2, a3, a4, a5, a6, a7) := bytes_from_word w in
-  let s := fun '(n, b) (m' : memory) => ZMap.set (Z.add (Word.intval addr) (Z.of_nat n)) b m' in
+  let s := fun '(n, b) (m' : memory) => mem_store_byte (wordadd addr n) b m' in
   fold_right s m [(7, a7); (6, a6); (5, a5); (4, a4); (3, a3); (2, a2); (1, a1); (0, a0)].
 
-Definition exec_mem_instr (i : mem_instruction) (m : memory) (ws : list word) : option (memory * list word) :=
-  match i, ws with
-    | I_MLOAD, addr::ws => Some (m, mem_read_word addr m :: ws )
-    | I_MSTORE, addr::val::ws => Some (mem_store_word addr val m, ws)
-    | I_MSTORE8, addr::val::ws => Some (mem_store_first_byte addr val m, ws)
-    | _, _ => None
-  end.
 
-Theorem exec_mem_nice : forall i m st m' st',
-  exec_mem_instr i m st = Some (m', st') ->
-    let d := delta (I_MEMINS i) in
-    let a := alpha (I_MEMINS i) in
-    st' = firstn a st' ++ skipn d st.
-Proof.
-  intros.
-  destruct (exec_mem_instr i m st) eqn:Q; inversion H.
-  subst.
-  destruct i; repeat (destruct st; inversion Q; try reflexivity).
-Qed.
+End Memory.
+
+Section Storage.
 
 Definition storage := WordMap.t word.
 
@@ -54,23 +48,32 @@ Definition storage_read (addr: word) (p: storage) : word := WordMap.get (Word.in
 
 Definition storage_store (addr: word) (w: word) (p: storage) : storage := WordMap.set (Word.intval addr) w p.
 
-(* storage should be indexed by contract id *)
-(* TODO: this is remarkably similar to the interface of CompCerts' Memory.v *)
-Definition exec_storage_instr (i : storage_instruction) (p : storage) (ws : list word) : option (storage * list word) :=
-  match i, ws with
-    | I_SLOAD, addr::ws => Some (p, storage_read addr p :: ws)
-    | I_SSTORE, addr::val::ws => Some (storage_store addr val p, ws)
-    | _, _ => None
-  end.
 
-Theorem exec_storage_nice : forall i p st p' st',
-  exec_storage_instr i p st = Some (p', st') ->
-    let d := delta (I_STORINS i) in
-    let a := alpha (I_STORINS i) in
-    st' = firstn a st' ++ skipn d st.
-Proof.
-  intros.
-  destruct (exec_storage_instr i p st) eqn:Q; inversion H.
-  subst.
-  destruct i; repeat (destruct st; inversion Q; try reflexivity).
-Qed.
+End Storage.
+
+
+Require Import Instructions.
+Require Import ZArith.Znat.
+
+Section Code.
+
+Definition code := memory.
+
+
+Definition pc_t := word.
+Definition inc_pc (pc : pc_t) : pc_t := add pc one.
+
+Definition code_read_byte := mem_read_byte.
+Definition code_read_word_from_n_bytes := mem_read_word_from_n_bytes.
+
+Definition code_read_instruction (pc: pc_t) (c: code) : instruction :=
+  nth (Z.to_nat (Byte.unsigned (code_read_byte pc c))) opcode I_INVALID.
+
+Local Definition addrseq (addr count : word) : list word :=
+  map (wordadd addr) (seq 0 (Z.to_nat (Word.unsigned count))).
+
+Definition copy_code_to_memory (c: code) (m: memory) (to from count : word) : memory :=
+  fold_right (fun '(t, f) m' => mem_store_byte t (code_read_byte f m) m') m (combine (addrseq from count) (addrseq to count)).
+
+
+End Code.
